src/Node.v
@@ -3,22 +3,22 @@ Require Import OrderedType.
 Require Import Classes.RelationClasses.
 
 Section Node.
-  Variables Name Storage : Type.
+  Variables Name Tag : Type.
   Inductive Node : Type :=
-  | file : Name -> Storage -> Node
+  | file : Name -> Tag -> Node
   | dir : Name -> list Node -> Node.
 End Node.
 
-Module Node_as_OT (N S:OrderedType) <: OrderedType.
+Module Node_as_OT (N T:OrderedType) <: OrderedType.
   Module MN := OrderedTypeFacts N.
-  Module MS := OrderedTypeFacts S.
+  Module MT := OrderedTypeFacts T.
 
-  Definition t := Node N.t S.t.
+  Definition t := Node N.t T.t.
 
   Definition eq (x1 x2 : t) : Prop :=
     match x1, x2 with
     | @dir _ _ n1 _, @dir _ _ n2 _ => N.eq n1 n2
-    | @file _ _ n1 s1, @file _ _ n2 s2 => N.eq n1 n2 /\ S.eq s1 s2
+    | @file _ _ n1 s1, @file _ _ n2 s2 => N.eq n1 n2 /\ T.eq s1 s2
     | _, _ => False
     end.
 
@@ -27,20 +27,20 @@ Module Node_as_OT (N S:OrderedType) <: OrderedType.
     | @dir _ _ n1 _, @dir _ _ n2 _ => N.lt n1 n2
     | @dir _ _ n1 _, @file _ _ n2 _ => N.lt n1 n2
     | @file _ _ n1 _, @dir _ _ n2 _ => N.lt n1 n2 \/ N.eq n1 n2
-    | @file _ _ n1 s1, @file _ _ n2 s2 => (N.lt n1 n2) \/ (N.eq n1 n2 /\ S.lt s1 s2)
+    | @file _ _ n1 s1, @file _ _ n2 s2 => (N.lt n1 n2) \/ (N.eq n1 n2 /\ T.lt s1 s2)
     end.
 
   Lemma eq_refl : Reflexive eq.
   Proof.
     hnf. destruct x; simpl.
-    - split; [apply N.eq_refl | apply S.eq_refl].
+    - split; [apply N.eq_refl | apply T.eq_refl].
     - apply N.eq_refl.
   Qed.
 
   Lemma eq_sym : Symmetric eq.
   Proof.
     hnf. intros. destruct x, y; simpl in *; try contradiction.
-    - destruct H. apply N.eq_sym in H. apply S.eq_sym in H0.
+    - destruct H. apply N.eq_sym in H. apply T.eq_sym in H0.
       split; assumption.
     - apply N.eq_sym in H. assumption.
   Qed.
@@ -48,7 +48,7 @@ Module Node_as_OT (N S:OrderedType) <: OrderedType.
   Lemma eq_trans : Transitive eq.
   Proof.
     hnf. intros. destruct x, y, z; simpl in *; try contradiction.
-    - destruct H, H0. split; [apply (N.eq_trans H H0) | apply (S.eq_trans H1 H2)].
+    - destruct H, H0. split; [apply (N.eq_trans H H0) | apply (T.eq_trans H1 H2)].
     - apply (N.eq_trans H H0).
   Qed.
 
@@ -75,7 +75,7 @@ Module Node_as_OT (N S:OrderedType) <: OrderedType.
     intros. destruct x, y, z; simpl_lt_cases.
     all: try assumption || (left; assumption) ||
              (right; split; [reflexivity | assumption]).
-    - assert (S.lt t1 t5); [revert H2 H1; apply S.lt_trans|].
+    - assert (T.lt t1 t5); [revert H2 H1; apply T.lt_trans|].
       right. split; assumption.
     - right. assumption.
   Qed.
@@ -85,7 +85,7 @@ Module Node_as_OT (N S:OrderedType) <: OrderedType.
     intros. unfold not; intro. destruct x, y; simpl in *; try contradiction.
     - destruct H, H0.
       + contradiction (N.lt_not_eq H).
-      + destruct H. contradiction (S.lt_not_eq H2).
+      + destruct H. contradiction (T.lt_not_eq H2).
     - contradiction (N.lt_not_eq H).
   Qed.
 
@@ -101,7 +101,7 @@ Module Node_as_OT (N S:OrderedType) <: OrderedType.
            apply GT; simpl; try assumption || (left; assumption)
          | _ => idtac
          end.
-    - destruct (S.compare t1 t3).
+    - destruct (T.compare t1 t3).
       + apply LT. simpl. right. split; assumption.
       + apply EQ. simpl. split; assumption.
       + apply GT. simpl. right. split; [apply (N.eq_sym e) | assumption].
@@ -113,7 +113,7 @@ Module Node_as_OT (N S:OrderedType) <: OrderedType.
   Definition eq_dec : forall (x y : t), {eq x y} + {~ eq x y}.
   Proof.
     intros. destruct x, y; simpl; try auto.
-    - case_eq (N.eq_dec t0 t2); case_eq (S.eq_dec t1 t3); intros;
+    - case_eq (N.eq_dec t0 t2); case_eq (T.eq_dec t1 t3); intros;
         try (left; split; assumption) ||
             (right; unfold not; intro; destruct H1; contradiction).
     - apply N.eq_dec.
